Sketched a new (unproved) semax_shortcut_logical, derived rule for && and || expressions; used it in verif_logical_compare which now builds nicely.

progs/verif_logical_compare.v
@@ -1,23 +1,107 @@
 Require Import floyd.proofauto.
 Require Import progs.logical_compare.
+Instance CompSpecs : compspecs := compspecs_program prog.
+Instance CS_legal : compspecs_legal CompSpecs.
+Proof. prove_CS_legal. Qed.
 
 Local Open Scope logic.
+
+
+(****  START *)
+
+Definition logical_and_result v1 v2 : int :=
+   if Int.eq v1 Int.zero then Int.zero else v2.
+
+Definition logical_or_result v1 v2 : int :=
+  if Int.eq v1 Int.zero then v2 else Int.one.
+
+Fixpoint quick_shortcut_logical (s: statement) : option ident :=
+match s with
+| Sifthenelse _ 
+     (Sset id (Econst_int _ (Tint I32 Signed {| attr_volatile := false; attr_alignas := None |})))
+     s2 => match quick_shortcut_logical s2 with None => None | Some id2 =>
+                 if ident_eq id id2 then Some id else None
+                end
+| Sifthenelse e1 s2
+     (Sset id (Econst_int _ (Tint I32 Signed {| attr_volatile := false; attr_alignas := None |})))
+      => match quick_shortcut_logical s2 with None => None | Some id2 =>
+                 if ident_eq id id2 then Some id else None
+            end
+| Sset id (Ecast _ (Tint IBool Unsigned {| attr_volatile := false; attr_alignas := None |})) =>
+        Some id
+| _ => None
+end.
+
+Fixpoint shortcut_logical (eval: expr -> option val) (tid: ident) (s: statement) 
+            : option (int * list expr) :=
+match s with
+| Sifthenelse e1 
+     (Sset id (Econst_int one (Tint I32 Signed {| attr_volatile := false; attr_alignas := None |})))
+     s2 => if andb (eqb_ident id tid) (Int.eq one Int.one)
+                then match eval e1 with
+                        | Some (Vint v1) => 
+                           match shortcut_logical eval tid s2 with
+                           | Some (v2, el) => Some (logical_or_result v1 v2, e1 :: el)
+                           | _ => None
+                           end 
+                        | _ => None 
+                        end
+                else None
+| Sifthenelse e1 s2
+     (Sset id (Econst_int zero (Tint I32 Signed {| attr_volatile := false; attr_alignas := None |})))
+      => if andb (eqb_ident id tid) (Int.eq zero Int.zero)
+            then match eval e1 with
+                     | Some (Vint v1) => 
+                      match shortcut_logical eval tid s2 with
+                      | Some (v2, el) => Some (logical_and_result v1 v2, e1 :: el)
+                      | _ => None
+                      end
+                   | _ => None
+                end
+            else None
+| Sset id (Ecast e (Tint IBool Unsigned {| attr_volatile := false; attr_alignas := None |})) =>
+        if eqb_ident id tid 
+        then match eval (Ecast e tbool) with
+                 | Some (Vint v) => Some (v, (Ecast e tbool :: nil))
+                 | _ => None 
+                end
+        else None
+| _ => None
+end.
+
+Lemma semax_shortcut_logical:
+  forall Espec Delta P Q R tid s v Qtemp Qvar el,
+   quick_shortcut_logical s = Some tid ->
+   typeof_temp Delta tid = Some tint ->
+   local2ptree Q Qtemp Qvar nil nil ->
+   Qtemp ! tid = None ->
+   shortcut_logical (msubst_eval_expr Delta Qtemp Qvar) tid s = Some (v, el) ->
+   PROPx P (LOCALx (tc_environ Delta :: Q) (SEPx R)) |-- fold_right (fun e q => tc_expr Delta e && q) TT el ->
+   @semax Espec Delta (PROPx P (LOCALx Q (SEPx R)))
+          s (normal_ret_assert (PROPx P (LOCALx (temp tid (Vint v) :: Q) (SEPx R)))).
+Admitted.
+
+(***** END *)
 
 Definition do_or_spec :=
  DECLARE _do_or
   WITH a: int, b : int
   PRE [ _a OF tbool, _b OF tbool ]
-         PROP () LOCAL (`(eq (Vint a)) (eval_id _a); `(eq (Vint b)) (eval_id _b)) SEP (TT)
+        PROP () LOCAL (temp _a (Vint a); temp _b (Vint b)) SEP ()
   POST [ tbool ]  
-        local(`eq retval `(logical_or_result tbool (Vint a) tbool (Vint b))).
+        PROP() LOCAL (temp ret_temp (Vint (logical_or_result a b)))
+        SEP().
+
 
 Definition do_and_spec :=
  DECLARE _do_and
   WITH a: int, b : int
   PRE [ _a OF tbool, _b OF tbool ]
-         PROP () LOCAL (`(eq (Vint a)) (eval_id _a); `(eq (Vint b)) (eval_id _b)) SEP (TT)
+        PROP () LOCAL (temp _a (Vint a); temp _b (Vint b)) SEP ()
   POST [ tbool ]  
-        local(`eq retval `(logical_and_result tbool (Vint a) tbool (Vint b))).
+        PROP() LOCAL (temp ret_temp (Vint (logical_and_result a b)))
+        SEP().
+
 
 Definition main_spec :=
  DECLARE _main
@@ -30,38 +114,21 @@ Definition Vprog : varspecs := nil.
 Definition Gprog : funspecs := 
     do_or_spec :: do_and_spec :: main_spec::nil.
 
-Lemma or_one_zero :
-forall r a b, 
-Vint r = logical_or_result tbool (Vint a) tbool (Vint b) ->
-Vint (if Int.eq r Int.zero then Int.zero else Int.one) = Vint r.
-Proof.
-intros. unfold logical_or_result in *. simpl in *.
-if_tac in H. inv H. auto.
-if_tac in H. inv H; auto.
-inv H. auto.
-Qed.
-
-Lemma and_one_zero :
-forall r a b, 
-Vint r = logical_and_result tbool (Vint a) tbool (Vint b) ->
-Vint (if Int.eq r Int.zero then Int.zero else Int.one) = Vint r.
-Proof.
-intros. unfold logical_and_result in *. simpl in *.
-repeat if_tac in H; inv H; auto.
-Qed.
+Ltac do_semax_shortcut_logical := 
+ eapply semax_shortcut_logical; 
+   [ reflexivity | reflexivity | prove_local2ptree 
+   | reflexivity | reflexivity
+   | unfold fold_right; entailer  ].
 
 Lemma body_do_or: semax_body Vprog Gprog f_do_or do_or_spec.
 Proof.
 start_function.
 name a_ _a.
 name b_ _b.
+
+eapply semax_seq'; [do_semax_shortcut_logical | abbreviate_semax].
 forward.
-entailer!.
-apply orp_right2. auto.
-forward. rewrite <- H.
-split.
-if_tac; auto.
-eapply or_one_zero; eauto.
+destruct TC,TC0; subst; entailer!.
 Qed.
 
 Lemma body_do_and: semax_body Vprog Gprog f_do_and do_and_spec.
@@ -69,24 +136,15 @@ Proof.
 start_function.
 name a_ _a.
 name b_ _b.
+eapply semax_seq'; [do_semax_shortcut_logical | abbreviate_semax].
 forward.
-entailer!.
-apply orp_right2. auto.
-forward. rewrite <- H.
-split.
-if_tac; auto. 
-eapply and_one_zero; eauto.
+destruct TC,TC0; subst; entailer!.
 Qed.
 
 Lemma body_main:  semax_body Vprog Gprog f_main main_spec.
 Proof.
 start_function.
 forward.
-unfold main_post.
-unfold TT. 
-simpl.
-apply prop_right.
-auto.
 Qed.
 
 Existing Instance NullExtension.Espec.
